main/hl/solutions/lean/HL/Hoare2.lean
@@ -3015,4 +3015,4 @@ theorem hoare_havoc_weakest (p q : Assertion) (x : Ident)
 
 end HimpHoare2
 
--- Source revision: 5c6e636, committed 2026-09-20 21:46 UTC
+-- Source revision: dcf4433, committed 2026-09-24 17:39 UTC
