main/hl/student/lean/HL.lean
@@ -5,4 +5,4 @@ import HL.Equiv
 import HL.Hoare
 import HL.Hoare2
 
--- Source revision: 5c6e636, committed 2026-09-20 21:46 UTC
+-- Source revision: dcf4433, committed 2026-09-24 17:39 UTC
