main/hl/student/lean/HL/Preface.lean
@@ -68,4 +68,4 @@ import SFLCompat
 --  was supported, in part, by the National Science Foundation under the
 --  NSF Expeditions grant 1521523, *The Science of Deep Specification*.
 
--- Source revision: 5c6e636, committed 2026-09-20 21:46 UTC
+-- Source revision: dcf4433, committed 2026-09-24 17:39 UTC
