main/lf/solutions/lean/LF.lean
@@ -11,4 +11,4 @@ import LF.Automation
 import LF.Typeclasses
 import LF.Postscript
 
--- Source revision: 5c6e636, committed 2026-09-20 21:46 UTC
+-- Source revision: dcf4433, committed 2026-09-24 17:39 UTC
