main/lf/solutions/lean/LF/Logic.lean
@@ -1436,15 +1436,6 @@ theorem identity {a : Prop} : a → a := fun h => h
 
 --   ----------------------------------------
 
---  As an aside, some tactics that accept an `at` clause can target several
---  locations at once, including the goal, written using the `⊢` symbol, by
---  listing them together after `at` — for instance, both `rw` and `dsimp`
---  support this.
-
-example (n m : Nat) (h : n + 0 = m) : n = m + 0 := by
-  rw [Nat.add_zero] at h ⊢
-  assumption
-
 --  ## Working with Decidable Properties
 
 --  We've seen two different ways of expressing logical claims in Lean:
@@ -2399,4 +2390,4 @@ theorem cm_peirce : ConsequentiaMirabilis → Peirce := by
 theorem peirce_cm : Peirce → ConsequentiaMirabilis := by
   intro h a; exact h a False
 
--- Source revision: 5c6e636, committed 2026-09-20 21:46 UTC
+-- Source revision: dcf4433, committed 2026-09-24 17:39 UTC
