main/lf/solutions/lean/LF/Preface.lean
@@ -419,4 +419,4 @@ import SFLCompat
 --  Note to developers (Benjamin Pierce @bcpierce00):
 --      Other funding should be acknowledged here...
 
--- Source revision: 5c6e636, committed 2026-09-20 21:46 UTC
+-- Source revision: dcf4433, committed 2026-09-24 17:39 UTC
