main/lf/student/lean/LF/Basics.lean
@@ -2108,4 +2108,4 @@ theorem inspectBag_changeBag_comm_ticketed
 end Airport
 end NatPlayground
 
--- Source revision: 5c6e636, committed 2026-09-20 21:46 UTC
+-- Source revision: dcf4433, committed 2026-09-24 17:39 UTC
