main/lf/terse/lean/LF/Basics.lean
@@ -979,4 +979,4 @@ theorem and3_exchange (b c d : Bool) :
 
 end Nat
 
--- Source revision: 5c6e636, committed 2026-09-20 21:46 UTC
+-- Source revision: dcf4433, committed 2026-09-24 17:39 UTC
