main/lf/terse/lean/LF/Logic.lean
@@ -933,13 +933,6 @@ namespace FunctionTheoremQuiz
 
 end FunctionTheoremQuiz
 
---  Aside: some tactics, like `rw` and `dsimp`, can list
---  several locations at once with `at`, including the goal:
-
-example (n m : Nat) (h : n + 0 = m) : n = m + 0 := by
-  rw [Nat.add_zero] at h ⊢
-  assumption
-
 --  ## Working with Decidable Properties
 
 --  We've seen two different ways of expressing logical
@@ -1346,4 +1339,4 @@ def ExcludedMiddle := ∀ a : Prop, a ∨ ¬ a
 --  Output:
 --    Classical.em (p : Prop) : p ∨ ¬p
 
--- Source revision: 5c6e636, committed 2026-09-20 21:46 UTC
+-- Source revision: dcf4433, committed 2026-09-24 17:39 UTC
