main/lf/terse/lean/LF/Poly.lean
@@ -687,4 +687,4 @@ def fold_plus : List Nat → Nat → Nat :=
 --  Output:
 --    fold_plus : List Nat → Nat → Nat
 
--- Source revision: 5c6e636, committed 2026-09-20 21:46 UTC
+-- Source revision: dcf4433, committed 2026-09-24 17:39 UTC
