main/lf/terse/lean/LF/Postscript.lean
@@ -68,4 +68,4 @@ import SFLCompat
 --    develops formalized mathematics using Lean and
 --    Mathlib.
 
--- Source revision: 5c6e636, committed 2026-09-20 21:46 UTC
+-- Source revision: dcf4433, committed 2026-09-24 17:39 UTC
