main/lf/terse/lean/LF/Preface.lean
@@ -488,4 +488,4 @@ import SFLCompat
 --  National Science Foundation under the NSF Expeditions
 --  grant 1521523, *The Science of Deep Specification*.
 
--- Source revision: 5c6e636, committed 2026-09-20 21:46 UTC
+-- Source revision: dcf4433, committed 2026-09-24 17:39 UTC
