main/ts/solutions/lean/TS.lean
@@ -7,4 +7,4 @@ import TS.StlcProp
 import TS.MoreStlc
 import TS.Sub
 
--- Source revision: 5c6e636, committed 2026-09-20 21:46 UTC
+-- Source revision: dcf4433, committed 2026-09-24 17:39 UTC
