main/ts/solutions/lean/TS/Stlc.lean
@@ -1450,4 +1450,4 @@ example : ¬ ∃ S T, <{ ∅ ⊢ λ x : ~S . x x ⦂ ~T }> := by
 
 end Stlc
 
--- Source revision: 5c6e636, committed 2026-09-20 21:46 UTC
+-- Source revision: dcf4433, committed 2026-09-24 17:39 UTC
