main/ts/student/lean/TS/MoreStlc.lean
@@ -2160,4 +2160,4 @@ theorem preservation (t t' : Tm) (τ : Ty)
 
 end StlcExtended
 
--- Source revision: 5c6e636, committed 2026-09-20 21:46 UTC
+-- Source revision: dcf4433, committed 2026-09-24 17:39 UTC
