main/ts/student/lean/TS/Sub.lean
@@ -1936,4 +1936,4 @@ end FormalThoughtExercises
 
 end StlcSub
 
--- Source revision: 5c6e636, committed 2026-09-20 21:46 UTC
+-- Source revision: dcf4433, committed 2026-09-24 17:39 UTC
