main/ts/terse/lean/TS/Slang.lean
@@ -416,4 +416,4 @@ end Slang.AevalRExtended
 --  Functional: computation. Relational: expressive. Best:
 --  both, proved equivalent.
 
--- Source revision: 5c6e636, committed 2026-09-20 21:46 UTC
+-- Source revision: dcf4433, committed 2026-09-24 17:39 UTC
