main/ts/terse/lean/TS/Sub.lean
@@ -1255,4 +1255,4 @@ theorem preservation {t t' : Tm} {τ : Ty}
 
 end StlcSub
 
--- Source revision: 5c6e636, committed 2026-09-20 21:46 UTC
+-- Source revision: dcf4433, committed 2026-09-24 17:39 UTC
